---
title: "Lecture 5"
date: 2026-02-03
---

## Most Probable Distribution

Picking up where we left off last time, we have a supersystem with 4 subsystems ($\eta = 4$) where each subsystem can be in one of three energy states ($E_1$, $E_2$, $E_3$). We created a system $\set{n}_1\rightarrow n_1=1, n_2=2, n_3=1$. For this set of occupation numbers we found a multiplicity $\Omega = 12$. 

Now we consider a second system $\set{n}_2$ with the occupation numbers: $n_1 = 2, n_2=0, n_3=2$. We can calculate the multiplicity of this using the formula from last lecture and find $\Omega = 6$.

What is the probability of observing $E_3$ in $\set{n}_1$? To find this we divide the number of systems in the desired energy level by the number of systems total

$$\frac{n_3}{\eta} = \frac{1}{4}$$

We can similarly find the probability of $E_3$ in $\set{n}_2$

$$\frac{n_3}{\eta} = \frac{2}{4} = \frac{1}{2}$$

We have found the probability of a a system being in the state $E_3$ in both $\set{n}_1$ and $\set{n}_2$ individually. Now we want to know the overall probability over both $\set{n}_1$ and $\set{n}_2$.

$$P_3 = \frac{\bar{n}}{\eta} = \frac{1}{\eta} \frac{\sum_n{\Omega (N) n_j}}{\sum_n{\Omega(n)}}$$

$$P_3 = \frac{1}{4} \left[ \frac{[12(1)+6(2)]}{12+6} \right] \longrightarrow \frac{1}{3}$$

Once we have the probability of each quantum state, we can find average properties, $\bar{M}$ using 

$$\bar{M} = \sum_j{M_j P_j}$$

However, the definition of $P_j$ makes this very difficult to calculate as $N \rightarrow \infty$. To avoid this difficulty we intrude another trick. If we let $\eta \rightarrow \infty$, we can take advance of the fact that the multi-nomial coefficient will begin to resemble a delta function where only the most probable value contributes to the overall distribution. We call this value $n^*$ (*The \* indicates that this is the most probable value of n, not a complex conjugate*)

As $\eta \rightarrow \infty$ all $\Omega(n)$ become negligible except $\Omega(n^*)$

$$P_j = \frac{\bar{n_j}}{\eta} =\frac{1}{\eta} \left[ \frac{\sum_n{\Omega (N) n_j(n^*)}}{\sum_n{\Omega(n)}} \right] \rightarrow \frac{1}{\eta} \left[ \frac{\Omega (n^*) n_j(n^*)}{\Omega(n^*)} \right] = \frac{n_j^*}{\eta}$$

Now we see that to find $P_j$ we only need to find the distribution that maximizes multiplicity. We can do this maximization using lagrange multipliers

## Constrained Optimization of Multiplicity

Constraints:

$$
\sum_j n_j = \eta
$$

$$
\sum_j n_j E_j = E_{\text{total}}
$$

First we look at the function we want to maximize:

$$
\Omega(n) = \frac{\eta!}{\prod_i n_i!}
$$

Using Stirling's approximation and some algebra we can change the form of this equation to

$$\ln \Omega(n) = \left[ \eta \ln \eta - \eta \right] - \left[ \sum_i (n_i \ln n_i - n_i) \right]$$

In this equation, the first term comes from the numerator and the second term comes from the denominator, since dividing inside a logarithm is equivalent to subtracting logarithms. We now distribute the negative sign through the second term and separate the summation:

$$\ln \Omega(n) = \left[ \eta \ln \eta - \eta \right] - \sum_i n_i \ln n_i + \sum_i n_i$$

Since $\sum_i n_i = \eta$, the final term cancels with the $-\eta$ in the first bracket, leaving

$$\ln \Omega(n) = \eta \ln \eta - \sum_i n_i \ln n_i$$

Using the constraint $\eta = \sum_i n_i$, this can be rewritten as

$$\ln \Omega(n) = \left( \sum_i n_i \right) \ln\!\left( \sum_i n_i \right)- \sum_i n_i \ln n_i$$

To maximize $\ln \Omega(n)$, we must take the derivative with respect to $n_i$ subject to the constraints on total particle number and total energy. We enforce these constraints using Lagrange multipliers $\alpha$ and $\beta$.

We therefore define the function

$$\Phi = \ln \Omega(n) - \alpha \left( \sum_i n_i - \eta \right) - \beta \left( \sum_i n_i E_i - E_{\text{total}} \right)$$

and require

$$\frac{\partial \Phi}{\partial n_i} = 0$$

Taking the derivative term by term gives

$$\frac{\partial}{\partial n_i} \left[\sum_j n_j \ln\!\left( \sum_j n_j \right) - \sum_j n_j \ln n_j \right] - \alpha - \beta E_i = 0$$

Evaluating the derivatives,

$$ \frac{\partial}{\partial n_i} \left[ \sum_j n_j \ln\!\left( \sum_j n_j \right) \right] = \ln\!\left( \sum_j n_j \right) + 1$$

and

$$ \frac{\partial}{\partial n_i} \left[ \sum_j n_j \ln n_j \right] = \ln n_i + 1$$

Substituting these results yields

$$ \left[ \ln\!\left( \sum_j n_j \right) + 1 \right]- \left[ \ln n_i + 1 \right] - \alpha - \beta E_i = 0$$

The constant terms cancel, leaving

$$\ln\!\left( \sum_j n_j \right) - \ln n_i = \alpha + \beta E_i$$

Combining the logarithms gives

$$\ln\!\left( \frac{\sum_j n_j}{n_i} \right) = \alpha + \beta E_i$$

Exponentiating both sides,

$$\frac{\sum_j n_j}{n_i} = e^{\alpha + \beta E_i}$$

or equivalently,

$$ n_i = \left( \sum_j n_j \right) e^{-\alpha} e^{-\beta E_i} $$

Since $\sum_j n_j = \eta$, this becomes

$$n_i = \eta \, e^{-\alpha} e^{-\beta E_i}$$

To determine the normalization constant, we sum over all states:

$$ \sum_i n_i = \eta \, e^{-\alpha} \sum_i e^{-\beta E_i} = \eta$$

Canceling $\eta$ from both sides gives

$$ e^{-\alpha} \sum_i e^{-\beta E_i} = 1$$

which implies

$$ e^{\alpha} = \sum_i e^{-\beta E_i}$$

This $e^{\alpha}$ is the "*canonical partition function $Q(N,V,\beta)$*"

Now $P_j$ does not involve the multiplicity of all distributions, only $n_j^*$ which maximizes $\Omega$.

$$P_j = \frac{n_j^*}{\eta} \rightarrow e^{-\alpha} e^{-\beta E_J} \rightarrow \frac{e^{-\beta E_j}}{Q}$$

$$\bar{E} = \sum_j{E_j P_j} = \frac{\sum_j [E_j e^{-\beta E_j}]}{Q}$$

We can find energy values using quantum mechanics and find the probability of each state. We can similarly find the pressure ofa. particular state $j$ from $PV$ work 

$$dE_j = -P_j dV \rightarrow P_j = \left( \frac{dE_j}{dV} \right)_N$$

$$\bar{p} = \sum_J{[p_j P_j]} = \frac{- \sum_j [\left( \frac{dE_j}{dV} \right)_N e^{-\beta E_j}]}{Q}$$

Now we still need to define the parameter $\beta$. To do this we recall $\bar{E} = \sum_j{E_j P_j}$ so 

$$d\bar{E} = \sum_j{\left[ E_j dP_j + P_j dE_j \right]}$$

## Canonical Ensemble Derivation

 Average pressure

$$\bar{P} = \sum_j P_j \, p_j$$


We still have not defined beta 

Define the average energy:

$$\bar{E} = \sum_j E_j p_j$$

Take the total differential:

$$d\bar{E} = \sum_j E_j \, dp_j + \sum_j p_j \, dE_j$$

Canonical probabilities

we can assume

$$p_j = \frac{e^{-\beta E_j}}{Q}$$

Then

$$\ln p_j = -\beta E_j - \ln Q$$

Solve for $E_j$:

$$E_j = -\frac{1}{\beta}\left( \ln p_j + \ln Q \right)$$

Substitute into $d\bar{E}$

$$ d\bar{E} = \sum_j \left[ -\frac{1}{\beta}(\ln Q + \ln p_j)\, dp_j + p_j \, dE_j \right]$$

Using mechanical work:

$$dE_j = -P_j \, dV$$

So

$$d\bar{E} = -\frac{1}{\beta}\sum_j (\ln Q + \ln p_j)\, dp_j+ \sum_j p_j(-P_j)\, dV$$

Simplifications

Normalization of probabilities:

$$\sum_j dp_j = 0$$

Thus the $\ln Q$ term vanishes:

$$d\bar{E}= -\frac{1}{\beta}\sum_j \ln p_j \, dp_j- \bar{P}\, dV$$

Entropy-like term

Use the identity:

$$\sum_j \ln p_j \, dp_j= d\!\left(\sum_j p_j \ln p_j\right)$$

Therefore:

$$d\bar{E}= -\frac{1}{\beta}d\!\left(\sum_j p_j \ln p_j\right)- \bar{P}\, dV$$

Rearranging:

$$d\bar{E} + \bar{P}\, dV= -\frac{1}{\beta}d\!\left(\sum_j p_j \ln p_j\right)$$

Thermodynamic identification

From the fundamental thermodynamic relation:

$$d\bar{E} + \bar{P}\, dV = T\, dS$$

Thus:

$$T\, dS= -\frac{1}{\beta}d\!\left(\sum_j p_j \ln p_j\right)$$

Which implies:

$$S = -k_B \sum_j p_j \ln p_j\qquad\beta = \frac{1}{k_B T}$$

Partition function and probabilities

$$Q(N,V,T)= \sum_j e^{-E_j(N,V)/k_B T}$$

$$p_j(N,V,T)= \frac{e^{-E_j(N,V)/k_B T}}{Q}$$

Helmholtz free energy

$$A = \bar{E} - T S$$

All thermodynamic quantities can be rewritten in terms of $Q$